adds reachable pc's and transitions

examples/spinlock/spinlock2Script.sml
@@ -8,10 +8,12 @@ val _ = set_trace "bir_inst_lifting.DEBUG_LEVEL" 2;
 
 val _ = new_theory "spinlock2";
 
+(*
 val (bir_spinlock_progbin_def, bir_spinlock_prog_def, bir_is_lifted_prog_spinlock) = lift_da_and_store_mc_riscv
           "spinlock"
           "spinlock.da"
           ((Arbnum.fromInt 0), (Arbnum.fromInt 0x1000000));
+*)
 
 open bir_promisingTheory rich_listTheory listTheory arithmeticTheory tracesTheory;
 open finite_mapTheory;
@@ -65,8 +67,8 @@ QED
 fun fun_eq_conjs term =
   let
     val ty = type_of term
-    val thm = 
-      ISPEC term ELIM_thms 
+    val thm =
+      ISPEC term ELIM_thms
       (* int_arithTheory.CONJ_EQ_ELIM *)
       |> SIMP_RULE (std_ss) []
   in
@@ -114,6 +116,11 @@ Theorem bir_get_stmt_bir_spinlock_prog_BirStmt_Expr =
   |> CONV_RULE CONJ_EQ_NEQ_conv
   |> GEN_ALL
 
+(*
+bir_get_stmt_bir_spinlock_prog_BirStmt_Write_EQ
+bir_get_stmt_bir_spinlock_prog_BirStmt_Read_EQ
+*)
+
 Theorem bir_get_stmt_bir_spinlock_prog_BirStmt_None =
   EVAL ``bir_get_stmt bir_spinlock_prog x = BirStmt_None``
   |> SIMP_RULE (srw_ss() ++ boolSimps.DNF_ss) [AllCaseEqs(),wordsTheory.NUMERAL_LESS_THM]
@@ -126,57 +133,324 @@ Definition init_def:
       ==> st.bst_pc = <| bpc_index := 0; bpc_label := BL_Address $ Imm64 0w |>
 End
 
-Theorem reachable_pc:
+(*
+  all possible steps with the spinlock
+  sl_step (blck,pc) (blck',pc')
+*)
+Inductive sl_step:
+  sl_step (BL_Address $ Imm64 x,y) (BL_Address $ Imm64 x,y)
+  /\ sl_step (BL_Address $ Imm64 0w,0n) (BL_Address $ Imm64 0w,1)
+  /\ sl_step (BL_Address $ Imm64 0w,1)  (BL_Address $ Imm64 4w,0)
+  /\ sl_step (BL_Address $ Imm64 4w,0)  (BL_Address $ Imm64 4w,1)
+  /\ sl_step (BL_Address $ Imm64 4w,1)  (BL_Address $ Imm64 8w,0)
+  /\ sl_step (BL_Address $ Imm64 8w,0)  (BL_Address $ Imm64 8w,1)
+  /\ sl_step (BL_Address $ Imm64 8w,1)  (BL_Address $ Imm64 12w,0)
+  /\ sl_step (BL_Address $ Imm64 12w,0) (BL_Address $ Imm64 12w,1)
+  /\ sl_step (BL_Address $ Imm64 12w,1) (BL_Address $ Imm64 12w,3)
+  /\ sl_step (BL_Address $ Imm64 12w,3) (BL_Address $ Imm64 16w,0)
+  /\ sl_step (BL_Address $ Imm64 16w,0) (BL_Address $ Imm64 12w,0)
+  /\ sl_step (BL_Address $ Imm64 16w,0) (BL_Address $ Imm64 20w,0)
+  /\ sl_step (BL_Address $ Imm64 20w,0) (BL_Address $ Imm64 20w,1)
+  /\ sl_step (BL_Address $ Imm64 20w,1) (BL_Address $ Imm64 20w,2)
+  /\ sl_step (BL_Address $ Imm64 20w,2) (BL_Address $ Imm64 20w,5)
+  /\ sl_step (BL_Address $ Imm64 20w,5) (BL_Address $ Imm64 24w,0)
+  /\ sl_step (BL_Address $ Imm64 24w,0) (BL_Address $ Imm64 12w,0)
+  /\ sl_step (BL_Address $ Imm64 24w,0) (BL_Address $ Imm64 28w,0)
+End
+
+Definition bst_pc_tuple_def:
+  bst_pc_tuple x = (x.bpc_label,x.bpc_index)
+End
+
+(*
+(*
+  TODO make this a function taking a term:
+  val term = ``sl_step``
+ *)
+val fun_snd_imp =
+  let
+    val values =
+      map (rand o concl o SPEC_ALL) $ CONJUNCTS sl_step_rules
+    val term' =
+      mk_imp (``sl_step å1 å2``,
+        map (fn value => mk_eq (``å2:bir_label_t # num``, value)) values
+        |> list_mk_disj)
+  in
+   prove(term', dsimp[sl_step_cases])
+  end
+*)
+
+Definition reachable_pc_def:
+  reachable_pc pc <=>
+    !bpt. bpt = bst_pc_tuple pc ==>
+    bpt = (BL_Address $ Imm64 0w,1) \/ bpt = (BL_Address $ Imm64 4w,0) \/
+    bpt = (BL_Address $ Imm64 4w,1) \/ bpt = (BL_Address $ Imm64 8w,0) \/
+    bpt = (BL_Address $ Imm64 8w,1) \/ bpt = (BL_Address $ Imm64 12w,0) \/
+    bpt = (BL_Address $ Imm64 12w,1) \/ bpt = (BL_Address $ Imm64 12w,3) \/
+    bpt = (BL_Address $ Imm64 16w,0) \/ bpt = (BL_Address $ Imm64 20w,0) \/
+    bpt = (BL_Address $ Imm64 20w,1) \/ bpt = (BL_Address $ Imm64 20w,2) \/
+    bpt = (BL_Address $ Imm64 20w,5) \/ bpt = (BL_Address $ Imm64 24w,0) \/
+    bpt = (BL_Address $ Imm64 28w,0) \/ bpt = (BL_Address $ Imm64 0w,0)
+End
+
+Theorem reachable_pc_sl_step_imp:
+  !pc pc'. reachable_pc pc
+  /\ sl_step (bst_pc_tuple pc) (bst_pc_tuple pc')
+  ==> reachable_pc pc'
+Proof
+  rw[reachable_pc_def]
+  >> gvs[sl_step_cases]
+QED
+
+Theorem reachable_pc_sim:
+  !i tr cid p st st'. wf_trace tr
+  /\ SUC i < LENGTH tr
+  /\ init (FST $ HD tr)
+  /\ core_runs_spinlock cid $ FST $ HD tr
+  /\ FLOOKUP (FST $ EL i tr) cid = SOME $ Core cid p st
+  /\ FLOOKUP (FST $ EL (SUC i) tr) cid = SOME $ Core cid p st'
+  /\ reachable_pc st.bst_pc
+  ==> sl_step (bst_pc_tuple st.bst_pc) (bst_pc_tuple st'.bst_pc)
+Proof
+  rpt gen_tac >> strip_tac
+  >> reverse $ Cases_on `parstep_nice cid (EL i tr) (EL (SUC i) tr)`
+  >- (
+    drule_all_then assume_tac wf_trace_NOT_parstep_nice_state_EQ'
+    >> fs[]
+    >> gvs[sl_step_rules,reachable_pc_def]
+  )
+  >> drule_all_then assume_tac wf_trace_core_runs_spinlock_FLOOKUP
+(* the remaining tactic mimick an EVAL for a parstep{_nice,} transition
+ * in the context of a concrete program 'bir_spinlock_prog'
+ * with the extracted possible pc locations of different instructions
+ * encoded in bir_get_stmt_bir_spinlock_prog_BirStmt_*
+ *)
+
+  >> fs[parstep_nice_def,parstep_cases,cstep_cases,FLOOKUP_UPDATE,clstep_cases,bir_programTheory.bir_pc_next_def,bst_pc_tuple_def,sl_step_cases]
+  >> gvs[FLOOKUP_UPDATE]
+  >> fs $ map (CONV_RULE (ONCE_DEPTH_CONV $ LHS_CONV SYM_CONV))
+    [bir_get_stmt_bir_spinlock_prog_BirStmt_Read_EQ,
+    bir_get_stmt_bir_spinlock_prog_BirStmt_Write_EQ,
+    bir_get_stmt_bir_spinlock_prog_BirStmt_Fence,
+    bir_get_stmt_bir_spinlock_prog_BirStmt_Generic,
+    bir_get_stmt_bir_spinlock_prog_BirStmt_Branch,
+    bir_get_stmt_bir_spinlock_prog_BirStmt_None,
+    bir_get_stmt_bir_spinlock_prog_BirStmt_Expr]
+  >> gvs[bir_programTheory.bir_pc_next_def,AllCaseEqs(),bir_get_stmt_bir_spinlock_prog_BirStmt_Write_EQ,bir_get_stmt_bir_spinlock_prog_BirStmt_Read_EQ,bir_get_stmt_bir_spinlock_prog_BirStmt_Expr,bir_get_stmt_bir_spinlock_prog_BirStmt_Generic,bir_get_stmt_bir_spinlock_prog_BirStmt_Expr,bir_get_stmt_bir_spinlock_prog_BirStmt_None,bir_get_stmt_bir_spinlock_prog_BirStmt_Branch,bir_programTheory.bir_exec_stmt_def,bir_programTheory.bir_exec_stmtB_def,bir_programTheory.bir_exec_stmt_assert_def,bir_expTheory.bir_eval_exp_def,bir_expTheory.bir_eval_bin_pred_def,bir_expTheory.bir_eval_bin_exp_def,bir_programTheory.bir_state_set_typeerror_def,bir_programTheory.bir_exec_stmtE_def,bir_programTheory.bir_exec_stmt_jmp_def,bir_programTheory.bir_eval_label_exp_def,bir_programTheory.bir_exec_stmt_jmp_to_label_def,bir_programTheory.bir_block_pc_def,bir_programTheory.bir_exec_stmt_cjmp_def,bst_pc_tuple_def,reachable_pc_def]
+  >> BasicProvers.every_case_tac
+  >> gvs[bir_programTheory.bir_pc_next_def,AllCaseEqs(),bir_get_stmt_bir_spinlock_prog_BirStmt_Write_EQ,bir_get_stmt_bir_spinlock_prog_BirStmt_Read_EQ,bir_get_stmt_bir_spinlock_prog_BirStmt_Expr,bir_get_stmt_bir_spinlock_prog_BirStmt_Generic,bir_get_stmt_bir_spinlock_prog_BirStmt_Expr,bir_get_stmt_bir_spinlock_prog_BirStmt_None,bir_get_stmt_bir_spinlock_prog_BirStmt_Branch,bir_programTheory.bir_exec_stmt_def,bir_programTheory.bir_exec_stmtB_def,bir_programTheory.bir_exec_stmt_assert_def,bir_expTheory.bir_eval_exp_def,bir_expTheory.bir_eval_bin_pred_def,bir_expTheory.bir_eval_bin_exp_def,bir_programTheory.bir_state_set_typeerror_def,bir_programTheory.bir_exec_stmtE_def,bir_programTheory.bir_exec_stmt_jmp_def,bir_programTheory.bir_eval_label_exp_def,bir_programTheory.bir_exec_stmt_jmp_to_label_def,bir_programTheory.bir_block_pc_def,get_fulfil_args_def,get_read_args_def]
+QED
+
+Theorem wf_trace_reachable_pc:
   !i tr cid p st. wf_trace tr
   /\ i < LENGTH tr
   /\ init (FST $ HD tr)
   /\ core_runs_spinlock cid $ FST $ HD tr
   /\ FLOOKUP (FST $ EL i tr) cid = SOME $ Core cid p st
-  ==> st.bst_pc IN {
-    <|bpc_label := BL_Address (Imm64 0w); bpc_index := 0|>;
-    <|bpc_label := BL_Address (Imm64 0w); bpc_index := 1|>;
-    <|bpc_label := BL_Address (Imm64 4w); bpc_index := 0|>;
-    <|bpc_label := BL_Address (Imm64 4w); bpc_index := 1|>;
-    <|bpc_label := BL_Address (Imm64 8w); bpc_index := 0|>;
-    <|bpc_label := BL_Address (Imm64 8w); bpc_index := 1|>;
-    <|bpc_label := BL_Address (Imm64 12w); bpc_index := 0|>;
-    <|bpc_label := BL_Address (Imm64 12w); bpc_index := 1|>;
-    <|bpc_label := BL_Address (Imm64 12w); bpc_index := 3|>;
-    <|bpc_label := BL_Address (Imm64 16w); bpc_index := 0|>;
-    <|bpc_label := BL_Address (Imm64 20w); bpc_index := 0|>;
-    <|bpc_label := BL_Address (Imm64 20w); bpc_index := 1|>;
-    <|bpc_label := BL_Address (Imm64 20w); bpc_index := 2|>;
-    <|bpc_label := BL_Address (Imm64 20w); bpc_index := 5|>;
-    <|bpc_label := BL_Address (Imm64 24w); bpc_index := 0|>
-  }
+  ==> reachable_pc st.bst_pc
 Proof
   Induct
-  >- (rw[init_def] >> res_tac >> fs[])
-  >> rw[]
-  >> drule_all_then strip_assume_tac wf_trace_cid_backward1
-  >> first_x_assum $ drule_then $ drule_at_then Any assume_tac
-  >> drule_all_then assume_tac wf_trace_core_runs_spinlock_FLOOKUP
-  >> reverse $ Cases_on `parstep_nice cid (EL i tr) (EL (SUC i) tr)`
+  >> rpt strip_tac
   >- (
-    drule_all_then assume_tac wf_trace_NOT_parstep_nice_state_EQ'
-    >> gs[]
+    fs[init_def]
+    >> res_tac
+    >> fs[bst_pc_tuple_def,reachable_pc_def]
   )
-  >>  gvs[parstep_nice_def,parstep_cases,cstep_cases,FLOOKUP_UPDATE,clstep_cases,bir_get_stmt_bir_spinlock_prog_BirStmt_Fence]
-  >> map_every (imp_res_tac o (
-      CONV_RULE (ONCE_DEPTH_CONV $ LAND_CONV $ SYM_CONV)
-    ) o iffLR)
-    [bir_get_stmt_bir_spinlock_prog_BirStmt_Read_EQ,
-    bir_get_stmt_bir_spinlock_prog_BirStmt_Write_EQ,
-    bir_get_stmt_bir_spinlock_prog_BirStmt_Generic,
-    bir_get_stmt_bir_spinlock_prog_BirStmt_Branch,
-    bir_get_stmt_bir_spinlock_prog_BirStmt_Expr]
-  >> asm_rewrite_tac[]
-  >> simp[bir_programTheory.bir_pc_next_def,bir_programTheory.bir_programcounter_t_component_equality]
-  >> imp_res_tac bir_get_stmt_bir_spinlock_prog
-  >> gns[]
-  >> gvs[bir_programTheory.bir_exec_stmt_def,bir_programTheory.bir_exec_stmtE_def,bir_programTheory.bir_exec_stmt_cjmp_def,AllCaseEqs(),bir_programTheory.bir_state_set_typeerror_def,bir_programTheory.bir_programcounter_t_component_equality,bir_programTheory.bir_exec_stmt_jmp_def,bir_programTheory.bir_eval_label_exp_def,bir_programTheory.bir_exec_stmt_jmp_to_label_def,bir_labels_of_program_bir_spinlock_prog,bir_programTheory.bir_block_pc_def,get_fulfil_args_def,get_read_args_def,bir_programTheory.bir_exec_stmtB_def,bir_programTheory.bir_state_is_terminated_def,bir_programTheory.bir_exec_stmt_assert_def,bir_expTheory.bir_eval_exp_def,bir_programTheory.bir_pc_next_def]
-  >> BasicProvers.every_case_tac
-  >> gvs[bir_programTheory.bir_exec_stmt_def,bir_programTheory.bir_exec_stmtE_def,bir_programTheory.bir_exec_stmt_cjmp_def,AllCaseEqs(),bir_programTheory.bir_state_set_typeerror_def,bir_programTheory.bir_programcounter_t_component_equality,bir_programTheory.bir_exec_stmt_jmp_def,bir_programTheory.bir_eval_label_exp_def,bir_programTheory.bir_exec_stmt_jmp_to_label_def,bir_labels_of_program_bir_spinlock_prog,bir_programTheory.bir_block_pc_def,get_fulfil_args_def,get_read_args_def,bir_programTheory.bir_exec_stmtB_def,bir_programTheory.bir_state_is_terminated_def,bir_programTheory.bir_exec_stmt_assert_def,bir_expTheory.bir_eval_exp_def,bir_programTheory.bir_pc_next_def]
+  >> drule_all_then strip_assume_tac wf_trace_cid_backward1
+  >> first_x_assum $ drule_at_then (Pat `FLOOKUP _ _ = _`) assume_tac
+  >> gs[]
+  >> drule_all_then assume_tac reachable_pc_sim
+  >> dxrule_all reachable_pc_sl_step_imp
+  >> fs[]
+QED
+
+Theorem reachable_pc_sl_step:
+  !i tr cid p st st'. wf_trace tr
+  /\ SUC i < LENGTH tr
+  /\ init (FST $ HD tr)
+  /\ core_runs_spinlock cid $ FST $ HD tr
+  /\ FLOOKUP (FST $ EL i tr) cid = SOME $ Core cid p st
+  /\ FLOOKUP (FST $ EL (SUC i) tr) cid = SOME $ Core cid p st'
+  ==> sl_step (bst_pc_tuple st.bst_pc) (bst_pc_tuple st'.bst_pc)
+Proof
+  rpt strip_tac
+  >> rev_drule_at_then (Pat `FLOOKUP _ _ = _`) assume_tac wf_trace_reachable_pc
+  >> gs[]
+  >> drule_all_then irule reachable_pc_sim
+QED
+
+(* unique properties *)
+
+Definition unique_def:
+  unique fmap P =
+    !id id' x x'. FLOOKUP fmap id = SOME x /\ P x
+      /\ FLOOKUP fmap id' = SOME x' /\ P x'
+      ==> id = id'
+End
+
+Theorem FLOOKUP_NOT_unique_eq:
+  !P cores cid st st'. FLOOKUP cores cid = SOME st
+  /\ ~(P st) /\ ~(P st')
+  ==> unique (FUPDATE cores (cid,st')) P = unique cores P
+Proof
+  rw[unique_def,EQ_IMP_THM]
+  >- (
+    first_x_assum irule
+    >> dsimp[FLOOKUP_UPDATE,AllCaseEqs()]
+    >> conj_tac >> spose_not_then assume_tac >> gvs[]
+  )
+  >> gs[FLOOKUP_UPDATE,AllCaseEqs()]
+QED
+
+Theorem FLOOKUP_unique_eq:
+  FLOOKUP cores cid = SOME st
+  /\ P st /\ P st'
+  ==> unique (FUPDATE cores (cid,st')) P = unique cores P
+Proof
+  rw[unique_def,EQ_IMP_THM]
+  >- (
+    first_x_assum irule
+    >> dsimp[FLOOKUP_UPDATE,AllCaseEqs(),LEFT_AND_OVER_OR,RIGHT_AND_OVER_OR]
+    >> metis_tac[]
+  )
+  >> gs[FLOOKUP_UPDATE,AllCaseEqs()]
+QED
+
+(* invariant *)
+
+Definition in_crit_def:
+  in_crit (Core id p st) <=>
+    st.bst_pc = <|bpc_label := BL_Address (Imm64 28w); bpc_index := 0|>
+End
+
+Theorem in_crit_sl_step:
+  !cid p st st'.
+  sl_step (bst_pc_tuple st.bst_pc) (bst_pc_tuple st'.bst_pc)
+  /\ st.bst_pc <> st'.bst_pc
+  /\ ~(in_crit $ Core cid p st')
+  ==> ~(in_crit $ Core cid p st)
+Proof
+  rw[sl_step_cases,in_crit_def,bst_pc_tuple_def,bir_programTheory.bir_programcounter_t_component_equality]
+  >> gvs[]
+QED
+
+Definition invariant_def:
+  invariant cores = unique cores in_crit
+End
+
+Definition wf_trace1_def:
+  wf_trace1 tr =
+    !i cid cid' p st. i < LENGTH tr
+      /\ FLOOKUP (FST $ EL i tr) cid = SOME $ Core cid' p st
+      ==> cid = cid'
+End
+
+Theorem wf_trace1_FLOOKUP:
+  !tr i id x. wf_trace1 tr
+  /\ FLOOKUP (FST $ EL i tr) id = SOME x
+  /\ i < LENGTH tr
+  ==> ?p st. x = Core id p st
+Proof
+  rw[wf_trace1_def]
+  >> qmatch_assum_rename_tac `FLOOKUP _ _ = SOME x`
+  >> Cases_on `x`
+  >> res_tac
+  >> fs[]
+QED
+
+Theorem init_unique_in_crit_imp:
+  !i tr. wf_trace tr /\ wf_trace1 tr
+  /\ init (FST $ HD tr)
+  ==> invariant (FST $ HD tr)
+Proof
+  rw[init_def,invariant_def,unique_def,Excl"EL",GSYM EL,Excl"EL_restricted"]
+  >> drule_then drule wf_trace1_FLOOKUP
+  >> drule_then rev_drule wf_trace1_FLOOKUP
+  >> rw[wf_trace_NOT_NULL,LENGTH_NOT_NULL]
+  >> fs[in_crit_def]
+  >> qpat_x_assum `!cid p st. FLOOKUP _ _ = _ ==> _` imp_res_tac
+  >> gs[]
+QED
+
+Definition same_state_def:
+  same_state cid st1 st2 =
+    !p st.
+      FLOOKUP st1 cid = SOME $ Core cid p st
+      /\ FLOOKUP st2 cid = SOME $ Core cid p st
+End
+
+Theorem init_unique:
+  !i tr. wf_trace tr /\ wf_trace1 tr
+  /\ SUC i < LENGTH tr
+  /\ cores_run_spinlock $ FST $ HD tr
+  /\ init (FST $ HD tr)
+  /\ invariant (FST $ EL i tr)
+  ==> invariant (FST $ EL (SUC i) tr)
+Proof
+  rw[invariant_def]
+  >> drule_all_then strip_assume_tac wf_trace_parstep_EL
+  >> imp_res_tac parstep_nice_EX_FLOOKUP
+  >> drule_all_then strip_assume_tac parstep_nice_FLOOKUP
+  >> drule_all_then assume_tac wf_trace_core_runs_spinlock_FLOOKUP'
+  >> Cases_on `st.bst_pc = st'.bst_pc`
+  >- (
+    fs[unique_def,in_crit_def,parstep_nice_def,parstep_cases]
+    >> rw[FLOOKUP_UPDATE,DISJ_EQ_IMP]
+    >> spose_not_then assume_tac
+    >> gvs[FLOOKUP_UPDATE]
+    >> first_x_assum $ dxrule_at $ Pat `FLOOKUP _ _ = _`
+    >> disch_then $ dxrule_at $ Pat `FLOOKUP _ _ = _`
+    >> fs[in_crit_def]
+  )
+  >> rev_drule_all_then assume_tac reachable_pc_sl_step
+  >> reverse $ Cases_on `in_crit $ THE $ FLOOKUP (FST $ EL (SUC i) tr) cid`
+  >- (
+    Q.ISPEC_THEN `in_crit` rev_drule FLOOKUP_NOT_unique_eq
+    >> disch_then $ drule_at Any
+    >> gvs[optionTheory.option_CLAUSES,parstep_nice_def,parstep_cases,FLOOKUP_UPDATE]
+    >> disch_then irule
+    >> drule_then (drule_at Any) in_crit_sl_step
+    >> fs[]
+  )
+  >> gvs[sl_step_cases,bst_pc_tuple_def,in_crit_def,bir_programTheory.bir_programcounter_t_component_equality]
+  >> reverse $ Cases_on `
+    ?cid p st. FLOOKUP (FST $ EL i tr) cid = SOME $ Core cid p st
+    /\ in_crit $ Core cid p st
+    `
+  >- (
+    rw[unique_def,FLOOKUP_UPDATE]
+    >> spose_not_then assume_tac
+    >> fs[DISJ_EQ_IMP]
+    >> qmatch_assum_rename_tac `FLOOKUP _ id' = SOME $ xx` >> Cases_on `xx`
+    >> qmatch_assum_rename_tac `FLOOKUP _ id = SOME $ xx` >> Cases_on `xx`
+    >> drule_then imp_res_tac wf_trace1_FLOOKUP
+    >> gvs[]
+    >> drule_at Any wf_trace_cid_backward1
+    >> qpat_x_assum `FLOOKUP _ _ = SOME _` mp_tac
+    >> drule_at Any wf_trace_cid_backward1
+    >> rpt strip_tac
+    >> gvs[]
+    >> PRED_ASSUM is_forall imp_res_tac
+    >> `id <> cid /\ id' <> cid` by (
+      conj_tac
+      >> spose_not_then assume_tac
+      >> gvs[]
+      >> rev_dxrule_at (Pat $ `FLOOKUP _ _ = _`) wf_trace_unchanged
+      >> disch_then $ dxrule_at_then (Pat $ `FLOOKUP _ _ = _`) assume_tac
+      >> gvs[]
+      >> gs[bir_programTheory.bir_state_t_component_equality,bir_programTheory.bir_programcounter_t_component_equality,in_crit_def]
+    )
+    >> Cases_on `parstep_nice id (EL i tr) (EL (SUC i) tr)`
+    >- imp_res_tac parstep_nice_parstep_nice
+    >> Cases_on `parstep_nice id' (EL i tr) (EL (SUC i) tr)`
+    >- imp_res_tac parstep_nice_parstep_nice
+    >> ntac 2 $ dxrule_at (Pat `~parstep_nice _ _ _`) wf_trace_NOT_parstep_nice_state_EQ'
+    >> rpt strip_tac
+    >> rfs[]
+    >> gvs[]
+  )
+  >> fs[]
+  >> cheat
 QED
 
 val _ = export_theory();
